\documentclass{article}
\usepackage{amsthm}
\usepackage{amssymb}
\usepackage{pgf, tikz}
\usetikzlibrary{arrows, automata}
\begin{document}
\title{Homework 13}
\author{Will Boland}
\maketitle

\textbf{Question 1}\newline
A) 2 + 4 + 6 + 8 = 20\newline
B) 1 + 3 + 8 + 17 = 29\newline
C) ${1/1 + 1/2 + 1/3 = 11/6}$\newline
D) ${5 * 4 * 3 * 2 * 1 = 120}$\newline
E) ${(5 * 4 * 3 * 2 * 1)/(4 * 3 * 2 * 1) = 120/24}$\newline
F) ${100! / 99! = 100}$\newline
G) ${100!/98! = 9900}$\newline\newline

\textbf{Question 2}\newline
\textbf{A)} \textit{Proof} (induction on n)\newline
(Base step, n = 7)\newline
${3^7 = 2187 < 5040 = 7!}$\newline\newline
(induction step)\newline
assume that ${3^k < k!}$ for any natural number ${k}$ $\geq$ ${7}$\newline
(Goal: ${3^{k+1}<(k+1)!}$)\newline
${3^{k+1} = 3^k * 3}$\newline
${ < k! * 3}$\newline
Because ${k > 6}$, we know that ${ k + 1 > 3}$\newline
${k! * 3 < k! * (k+1)}$\newline
${ = (k + 1)!}$\newline
Therefore, ${3^{k+1}<(k+1)!}$ $\square$\newline\newline


\textbf{B)} \textit{Proof} (induction on n)\newline
(Base step, n = 2)\newline
${3^2 = 9 > 4 = 2^2}$\newline\newline
(induction step)\newline
assume that ${3^k > k^2}$ for any ${k}$ $\geq$ ${2}$\newline
(Goal: ${3^{k+1}>(k+1)^2}$)\newline
${3^{k+1} = 3^k * 3^1}$\newline
${ = 3^k * 3}$\newline
${ > k^2 * 3}$\newline
${ = k^2 + k^2 + k^2}$\newline
Since ${k}$ $\geq$ 2, ${k^2}$ $\geq$ 4\newline
${k^2 + k^2 + k^2 > (k+1) * (k+1) = (k+1)^2}$\newline
Therefore,  ${3^{k+1}>(k+1)^2}$ $\square$\newline\newline


\textbf{C)} \textit{Proof} (induction on n)\newline
(Base step, n = 1)\newline
$$\sum_{i=1}^{n} 2i = 2*1 = 2 = 1(1+1) = n(n+1)$$\newline\newline
(induction step)\newline
assume $\sum\limits_{i=1}^{k} 2i = k(k+1)$ for some natural number k $\geq$ 1\newline
 $$\sum_{i=1}^{k+1} 2i = (\sum_{i=1}^{k} 2i) + 2(k+1) = k(k+1) + 2(k+1)$$\newline
${k(k+1)+2(k+1) = k^2+k+2k+2 = k^2+3k+2 = (k+1)(k+2) = (k+1)((k+1) +1 )}$$\square$\newline\newline


\textbf{D)} \textit{Proof} (induction on n)\newline
(Base step, n = 1)\newline
$$\sum_{i=1}^{n} 2^{i-1} = 2^{1-1} = 2^0 = 1 = 2^1 - 1 = 2^n - 1$$\newline
(induction step)\newline
 $\sum\limits_{i=1}^{k} 2^{i-1} = 2^k - 1$ for some natural number k $\geq$ 1 \newline
$$\sum_{i=1}^{k+1} 2^{i-1} = (\sum_{i=1}^{k} 2^{i-1}) + 2^{(k+1) - 1} = 2^{k} - 1 + 2^{(k+1) - 1}$$\newline
${2^{k}-1+2^{(k+1) - 1} = 2^{k}-1+2^{k} = 2^{k+1} - 1}$ $\square$\newline\newline


\textbf{E)} \textit{Proof} (induction on n)\newline
(Base step, n = 1)\newline
$$\sum_{i=0}^{n} i! * i = 0! * 0 + 1! * 1 = 1 = (1 + 1)! - 1 = (n + 1)! - 1$$\newline
(induction step)\newline
$\sum\limits_{i=1}^{k} i! * i = (k + 1)! - 1$ for some natural number k\newline
$$\sum_{i=0}^{k+1} i! * i = (\sum_{i=0}^{k}) + (k+1)! * (k+1) = (k+1)!-1 + (k+1)! * (k+1)$$\newline
${(k+1)!-1+(k+1)!*(k+1) = (k+1)!(k+1)!(k+1)-1 = 2(k+1)!(k+1)-1 = (2k+2)!(k+1)-1 }$$\newline
$${= (2k^2+4k+2)!-1 = (k+2)!-1}$$\square$\newline\newline


\textbf{F)} \textit{Proof} (induction on n)\newline
(Base step, n = 1)\newline
${n^2 - 3n = 1^2 - 3(1) = 1 - 3 = -2 and -2 is even because -2 = 2(-1)}$\newline
(induction step)\newline
Assume that ${k^2 - 3k}$ is even for some natural number k. This means that ${k^2 - 3k = 2j}$ for some integer j.\newline
${(k+1)^2 - 3(k+1) = (k+1)(k+1) - 3(k+1)}$\newline
${ = (k+1)^2 -3k-3}$\newline
${ = k^2 + 2k + 1 -3k - 3}$\newline
${ = k^2 - 3k + 2k + 1 - 3}$\newline
${ = 2j + 2k - 2}$\newline
${ = 2(j + k - 1)}$\newline
Since j + k - 1 is an integer, this means that ${(k+1)^2 - 3(k+1)}$ is even. $\square$
\enddocument





\textbf{A)} \textit{Proof} (induction on n)\newline
(Base step, n = 7)\newline
${3^7 = 2187 < 5040 = 7!}$\newline\newline
(induction step)\newline
assume that ${3^k < k!}$ for any ${k}$ $\geq$ ${7}$\newline
(Goal: ${3^{k+1}<(k+1)!}$)\newline


