\documentclass{article}
\usepackage{amsthm}
\usepackage{amssymb}
\begin{document}
\title{Mini-Homework 3}
\author{Will Boland}
\maketitle

\textbf{Claim: This is valid}\newline
$\neg$$\neg$A $\wedge$ $\neg$B, A $\rightarrow$ C $\vdash$ C $\wedge$ $\neg$B\newline\newline

\textbf{\textit{Proof}}\newline
Assume $\neg$$\neg$A $\wedge$ $\neg$B and A $\rightarrow$ C.\newline
Since $\neg$$\neg$A $\wedge$ $\neg$ B,we know $\neg$$\neg$A and $\neg$B ($\wedge$-elimination)\newline
From $\neg$$\neg$A, we get A (Double negation)\newline
Applying A $\rightarrow$ C to A gives us C (Application, or $\rightarrow$-elim)\newline
Because C and $\neg$B, C $\wedge$ $\neg$B. ($\wedge$-introduction)$\square$

\end{document}