\documentclass{article}
\usepackage{amsthm}
\usepackage{amssymb}
\begin{document}
\title{Notes}
\author{Will Boland}
\maketitle

Commutative Laws\newline
p$\wedge$q $\equiv$ q$\wedge$p ($\wedge$-Commutative)\newline
p$\lor$q $\equiv$ q$\lor$p ($\lor$-Commutative)\newline\newline

Association Laws\newline
p$\wedge$(q$\wedge$r) $\equiv$ (p$\wedge$q)$\wedge$r\newline
p$\lor$(q$\lor$r) $\equiv$ (p$\lor$q)$\lor$r\newline\newline

DeMorgan's Laws\newline
$\neg$(p$\wedge$q) $\equiv$ $\neg$p$\lor$$\neg$q\newline
$\neg$(p$\lor$q) $\equiv$ $\neg$p$\wedge$$\neg$q\newline\newline

Distributive Laws\newline
p$\wedge$(q$\lor$r) $\equiv$ (p$\wedge$q)$\lor$(p$\wedge$r)\newline
p$\lor$(q$\wedge$r) $\equiv$ (p$\lor$q)$\wedge$(p$\lor$r)\newline\newline

Double Negation\newline
$\neg$$\neg$p $\equiv$ p \newline\newline

Idempotence Laws\newline
p$\wedge$p $\equiv$ p\newline
p$\lor$p $\equiv$ p\newline\newline

Absorption\newline
p$\wedge$(q$\lor$p) $\equiv$ p\newline\newline

Implication or Material Implication\newline
p$\rightarrow$q $\equiv$ $\neg$p$\lor$q\newline\newline

Bi-Implication\newline
p$\leftrightarrow$q $\equiv$ (p$\wedge$q)$\lor$($\neg$p$\wedge$$\neg$q)\newline\newline

Exclusive Disjunction\newline
p$\oplus$q $\equiv$ (p$\wedge$$\neg$q)$\lor$($\neg$p$\wedge$q)\newline

Equality is \underline{transitive} meaning that if x = y and y = z, then z = y.\newline
Because + is transitive, these chain proofs make sense.\newline\newline

\textbf{Claim: } (A$\wedge$B)$\lor$(C$\wedge$D) $\equiv$ (D$\wedge$C)$\lor$(B$\wedge$A)\newline

\textbf{\textit{Proof: }}\newline
(A$\wedge$B)$\lor$(C$\wedge$D) $\equiv$ (C$\wedge$D)$\lor$(A$\wedge$B) ($\lor$-Commutative)\newline
$\equiv$ (D$\wedge$C)$\lor$(A$\wedge$B) ($\wedge$-Commutative)\newline
$\equiv$ (D$\wedge$C)$\lor$(B$\wedge$A) ($\wedge$-Commutative)$\square$$\newline$$\newline$


\textbf{Claim: } X$\rightarrow$Y $\equiv$ $\neg$Y $\rightarrow$$\neg$X\newline

\textbf{\textit{Proof: }}\newline
X$\rightarrow$Y $\equiv$ $\neg$X$\lor$Y (Material implication)\newline
	$\equiv$ Y$\lor$$\neg$X ($\lor$-Comm.)\newline

$\neg$Y$\rightarrow$$\neg$X $\equiv$ $\neg$$\neg$Y$\lor$$\neg$X (Mat. Imp)\newline
	$\equiv$ Y$\lor$$\neg$X (double negation) $\square$\newline\newline


\textbf{DO NOT DO THIS:}\newline
Pf: \newline
X$\rightarrow$Y $\equiv$ $\neg$Y$\rightarrow$$\neg$X\newline
$\neg$X$\lor$Y $\equiv$ $\neg$$\neg$Y$\lor$$\neg$X\newline
$\neg$X$\lor$Y $\equiv$ Y$\lor$$\neg$X\newline
Y$\lor$$\neg$X $\equiv$ Y$\lor$$\neg$X$\square$\newline
\textbf{DO NOT START A PROOF BY STATING THAT YOUR CLAIM IS TRUE}\newline\newline\newline


\textbf{Claim: }(A$\rightarrow$B)$\rightarrow$C $\equiv$ A$\rightarrow$(B$\rightarrow$C)\newline

\textbf{\textit{Proof: }}\newline
(A$\rightarrow$B)$\rightarrow$C $\equiv$ $\neg$(A$\rightarrow$B)$\lor$C (imp.)\newline
	$\equiv$ $\neg$($\neg$A$\lor$B) (imp.)$\lor$C\newline
	$\equiv$ ($\neg$$\neg$A$\wedge$$\neg$B)$\lor$C (demorgan's)\newline
	$\equiv$ (A$\wedge$$\neg$B)$\lor$C (double neg)\newline

A$\rightarrow$(B$\rightarrow$C) $\equiv$ $\neg$A $\lor$ (B$\rightarrow$C) (imp.)\newline
	$\equiv$ $\neg$A$\lor$($\neg$B$\lor$C) (imp.)\newline
	$\equiv$ ($\neg$A$\lor$$\neg$B)$\lor$C (Assoc.)\newline
Not equivalent! (A=F, B=T , C=F)




\end{document}